     closed_form :  
     
       |-------
     \{1\}   (FORALL (n: nat): sum(n) = (n * (n + 1)) / 2)
     
     Rule? {\bf (induct "n")}
     Inducting on n,
     this yields  2 subgoals: 
     closed_form.1 :  
     
       |-------
     \{1\}   sum(0) = (0 * (0 + 1)) / 2
     
     Rule? {\bf (postpone)}
     Postponing closed_form.1.
     
     closed_form.2 :  
     
       |-------
     \{1\}   (FORALL (j: nat):
              sum(j) = (j * (j + 1)) / 2
                IMPLIES sum(j + 1) = ((j + 1) * (j + 1 + 1)) / 2)
     
     Rule? {\bf (postpone)}
     Postponing closed_form.2.
     
     closed_form.1 :  
     
       |-------
     \{1\}   sum(0) = (0 * (0 + 1)) / 2
     
     Rule? {\bf (expand "sum")}
     (IF 0 = 0 THEN 0 ELSE 0 + sum(0 - 1) ENDIF) 
     simplifies to 0
     Expanding the definition of sum,
     this simplifies to: 
     closed_form.1 :  
     
       |-------
     \{1\}   0 = 0 / 2
     
     Rule? {\bf (assert)}
     Simplifying, rewriting, and recording with decision procedures,
     
     This completes the proof of closed_form.1.
     
     closed_form.2 :  
     
       |-------
     \{1\}   (FORALL (j: nat):
              sum(j) = (j * (j + 1)) / 2
                IMPLIES sum(j + 1) = ((j + 1) * (j + 1 + 1)) / 2)
     
     Rule? {\bf (skolem!)}
     Skolemizing,
     this simplifies to: 
     closed_form.2  |-------
     \{1\}   sum(j!1) = (j!1 * (j!1 + 1)) / 2
             IMPLIES sum(j!1 + 1) = ((j!1 + 1) * (j!1 + 1 + 1)) / 2
     
     Rule? {\bf (flatten)}
     Applying disjunctive simplification to flatten sequent,
     this simplifies to: 
     closed_form.2 :  
     
     \{-1\}   sum(j!1) = (j!1 * (j!1 + 1)) / 2
       |-------
     \{1\}   sum(j!1 + 1) = ((j!1 + 1) * (j!1 + 1 + 1)) / 2
     
     Rule? {\bf (expand "sum" +)}
     (IF j!1 + 1 = 0 THEN 0 ELSE j!1 + 1 + sum(j!1 + 1 - 1) ENDIF) 
     simplifies to 1 + sum(j!1) + j!1
     Expanding the definition of sum,
     this simplifies to: 
     closed_form.2 :  
     
     [-1]   sum(j!1) = (j!1 * (j!1 + 1)) / 2
       |-------
     \{1\}   1 + sum(j!1) + j!1 = (2 + j!1 + (j!1 * j!1 + 2 * j!1)) / 2
     
     Rule? {\bf (assert)}
     Simplifying, rewriting, and recording with decision procedures,
     
     This completes the proof of closed_form.2.
     
     Q.E.D.
     
     
     Run time  = 5.62 secs.
     Real time = 58.95 secs.
